src/proofs/no_slashable_attestations/main_theorem.dfy
@@ -1,0 +1,59 @@
+include "../../common/commons.dfy"
+include "../../specs/dvn/dvn.dfy"
+
+include "supporting_lemmas/proofs_ind_inv.dfy"
+
+module No_Slashable_Attestations_Main_Theorem
+{
+    import opened Types 
+    import opened DV
+    import opened Proofs_DVN_Ind_Inv
+
+
+    predicate isValidTrace(
+        trace: iseq<DVState>
+    )  
+    {
+        && DV.Init(trace[0], {})
+        && (
+            forall i: nat ::
+                DV.NextPreCond(trace[i]) ==> DV.Next(trace[i], trace[i+1])
+        )
+    }  
+
+    lemma lemma_non_slashable_attestations_rec(
+        trace: iseq<DVState>,
+        i: nat
+    )
+    requires isValidTrace(trace)
+    ensures forall j | 0 <= j <= i ::
+        && NextPreCond(trace[j])  
+        && ind_inv(trace[j])
+    {
+        if i == 0 
+        {
+            lemma_ind_inv_dvn_init(trace[0]);
+        }
+        else 
+        {
+            lemma_non_slashable_attestations_rec(trace, i-1);
+            lemma_ind_inv_dvn_ind(trace[i-1], trace[i]);
+        }
+    }
+
+    lemma lemma_non_slashable_attestations(
+        trace: iseq<DVState>
+    )
+    requires isValidTrace(trace)
+    ensures forall i:nat :: non_slashable_attestations(trace[i])
+    {
+        forall i:nat
+        ensures ind_inv(trace[i])
+        ensures non_slashable_attestations(trace[i])
+        {
+            lemma_non_slashable_attestations_rec(trace, i);
+            lemma_ind_inv_4_1_general(trace[i]);
+        }
+        
+    }    
+}
